Lurk/New/Store.lean
@@ -1,0 +1,90 @@
+import Std.Data.RBMap
+import Lurk.New.Tag
+
+open Lurk (F)
+
+def hash2 : F → F → F :=
+  fun a b => a * b * b
+
+def hash3 : F → F → F → F :=
+  fun a b c => a * b * b * c * c * c
+
+def hash4 : F → F → F → F → F :=
+  fun a b c d => a * b * b * c * c * c * d * d * d * d
+ 
+def hash6 : F → F → F → F → F → F → F :=
+  fun a b c d e f => a * b * b * c * c * c * d * d * d * d * e * e * e * e * e
+    * f * f * f * f * f * f
+
+def hash8 : F → F → F → F → F → F → F → F → F :=
+  fun a b c d e f g h => a * b * b * c * c * c * d * d * d * d * e * e * e * e * e
+    * f * f * f * f * f * f * g * g * g * g * g * g * g
+    * h * h * h * h * h * h * h * h
+
+structure ExprPtr where
+  tag : ExprTag
+  val : F
+  deriving Ord, BEq
+
+structure ContPtr where
+  tag : ContTag
+  val : F
+  deriving Ord
+
+inductive ExprPtrImg
+  | cons : ExprPtr → ExprPtr → ExprPtrImg
+  | strCons : ExprPtr → ExprPtr → ExprPtrImg
+  | symCons : ExprPtr → ExprPtr → ExprPtrImg
+  | «fun» : ExprPtr → ExprPtr → ExprPtr → ExprPtrImg
+  | comm : F → ExprPtr → ExprPtrImg
+
+inductive ContPtrImg
+  | cont0 : ContPtr → ContPtrImg
+  | cont1 : ExprPtr → ContPtr → ContPtrImg
+  | cont2 : ExprPtr → ExprPtr → ContPtr → ContPtrImg
+  | cont3 : ExprPtr → ExprPtr → ExprPtr → ContPtr → ContPtrImg
+
+open Std (RBMap)
+
+inductive Symbol
+  | root
+  | cons : String → Symbol → Symbol
+  deriving Ord
+
+namespace Symbol
+
+def telescope (acc : List String := []) : Symbol → List String
+  | root => acc
+  | cons str sym => sym.telescope $ str :: acc
+
+def toString (sym : Symbol) : String :=
+  ".".intercalate sym.telescope
+
+instance : ToString Symbol := ⟨Symbol.toString⟩
+
+@[inline] def nil : Symbol :=
+  .cons "nil" .root
+
+@[inline] def t : Symbol :=
+  .cons "t" .root
+
+end Symbol
+
+structure Store where
+  exprData : RBMap ExprPtr ExprPtrImg compare
+  strs : RBMap ExprPtr String compare
+  syms : RBMap ExprPtr Symbol compare
+  strsMemo : RBMap String ExprPtr compare
+  symsMemo : RBMap Symbol ExprPtr compare
+
+  contData : RBMap ContPtr ContPtrImg compare
+
+namespace Store
+
+def getStr (store : Store) : ExprPtr → Except String String := sorry
+def getSym (store : Store) : ExprPtr → Except String Symbol := sorry
+
+def putStr (store : Store) : String → (ExprPtr × Store) := sorry
+def putSym (store : Store) : Symbol → (ExprPtr × Store) := sorry
+
+end Store
