Lurk/New/Tag.lean
@@ -1,0 +1,56 @@
+import Lurk.Field
+
+inductive ExprTag
+  | num | u64 | char | str | comm | «fun» | sym | cons
+  deriving Ord, BEq
+
+inductive UnOp
+  | car
+  deriving Ord, BEq
+
+inductive BinOp
+  | add
+  | numEq
+  deriving Ord, BEq
+
+inductive ContTag
+  | done
+  | unOp : UnOp → ContTag
+  | binOp₁ : BinOp → ContTag
+  | binOp₂ : BinOp → ContTag
+  | appFn | appArg
+  | «if»
+  | «let»
+  | letrec
+  deriving Ord, BEq
+
+open Lurk (F)
+
+def ExprTag.toF : ExprTag → F
+  | .num  => .ofNat 2
+  | .u64  => .ofNat 3
+  | .char => .ofNat 5
+  | .str  => .ofNat 7
+  | .comm => .ofNat 11
+  | .fun  => .ofNat 13
+  | .sym  => .ofNat 17
+  | .cons => .ofNat 19
+
+def ContTag.toF : ContTag → F
+  | .done => .ofNat 23
+  | .unOp .car => .ofNat 29
+  | .binOp₁ .add => .ofNat 31
+  | .binOp₁ .numEq => .ofNat 37
+  | .binOp₂ .add => .ofNat 41
+  | .binOp₂ .numEq => .ofNat 43
+  | .appFn => .ofNat 47
+  | .appArg => .ofNat 53
+  | .if => .ofNat 59
+  | .let => .ofNat 61
+  | .letrec => .ofNat 67
+
+theorem ExprTag.toF_inj {t₁ t₂ : ExprTag} (h : t₁ ≠ t₂) : t₁.toF ≠ t₂.toF := sorry
+
+theorem ContTag.toF_inj {t₁ t₂ : ContTag} (h : t₁ ≠ t₂) : t₁.toF ≠ t₂.toF := sorry
+
+theorem toF_disj {et : ExprTag} {ct : ContTag} : et.toF ≠ ct.toF := sorry
